WebAssembly/Wasm_Instantiation.thy
@@ -34,6 +34,7 @@ lemma alloc_func_length:
   assumes "alloc_func s m_f i = (s', i_f)"
   shows "length (funcs s) = i_f"
         "length (funcs s') = Suc i_f"
+        "\<exists>farb. (funcs s)@[farb] = (funcs s')"
         "(tabs s) = (tabs s')"
         "(mems s) = (mems s')"
         "(globs s) = (globs s')"
@@ -46,6 +47,7 @@ lemma alloc_tab_length:
   shows "length (tabs s) = i_t"
         "length (tabs s') = Suc i_t"
         "(funcs s) = (funcs s')"
+        "\<exists>tarb. (tabs s)@[tarb] = (tabs s')"
         "(mems s) = (mems s')"
         "(globs s) = (globs s')"
   using assms[symmetric]
@@ -58,6 +60,7 @@ lemma alloc_mem_length:
         "length (mems s') = Suc i_m"
         "(funcs s) = (funcs s')"
         "(tabs s) = (tabs s')"
+        "\<exists>marb. (mems s)@[marb] = (mems s')"
         "(globs s) = (globs s')"
   using assms[symmetric]
   unfolding alloc_mem_def
@@ -70,6 +73,7 @@ lemma alloc_glob_length:
         "(funcs s) = (funcs s')"
         "(tabs s) = (tabs s')"
         "(mems s) = (mems s')"
+        "(globs s)@[\<lparr>g_mut=(tg_mut (module_glob.g_type m_g)), g_val=v\<rparr>] = (globs s')"
   using assms[symmetric]
   unfolding alloc_glob_def
   by (simp_all split: prod.splits)
@@ -77,6 +81,7 @@ lemma alloc_glob_length:
 lemma alloc_funcs_range:
   assumes "alloc_funcs s m_fs i = (s', i_fs)"
   shows "i_fs = [length (funcs s) ..< (length (funcs s) + length m_fs)] \<and>
+         (\<exists>farb. (funcs s)@farb = (funcs s')) \<and>
          (tabs s) = (tabs s') \<and>
          (mems s) = (mems s') \<and>
          (globs s) = (globs s')"
@@ -94,13 +99,16 @@ next
     by (simp split: prod.splits)
   thus ?case
     using Cons(1)[OF s''_is(2)] using alloc_func_length[OF s''_is(1)] upt_rec
-    by (simp split: prod.splits if_splits)    
+    apply (simp split: prod.splits)
+    apply (metis append_assoc)
+    done
 qed
 
 lemma alloc_tabs_range:
   assumes "alloc_tabs s m_ts = (s', i_ts)"
   shows "i_ts = [length (tabs s) ..< (length (tabs s) + length m_ts)] \<and>
          (funcs s) = (funcs s') \<and>
+         (\<exists>tarb. (tabs s)@tarb = (tabs s')) \<and>
          (mems s) = (mems s') \<and>
          (globs s) = (globs s')"
   using assms
@@ -117,7 +125,9 @@ next
     by (simp split: prod.splits)
   thus ?case
     using Cons(1)[OF s''_is(2)] using alloc_tab_length[OF s''_is(1)] upt_rec
-    by (simp split: prod.splits if_splits)
+    apply (simp split: prod.splits)
+    apply (metis append_assoc)
+    done
 qed
 
 lemma alloc_mems_range:
@@ -125,6 +135,7 @@ lemma alloc_mems_range:
   shows "i_ms = [length (mems s) ..< (length (mems s) + length m_ms)] \<and>
          (funcs s) = (funcs s') \<and>
          (tabs s) = (tabs s') \<and>
+         (\<exists>marb. (mems s)@marb = (mems s')) \<and>
          (globs s) = (globs s')"
   using assms
 proof (induction m_ms arbitrary: s i_ms)
@@ -140,7 +151,9 @@ next
     by (simp split: prod.splits)
   thus ?case
     using Cons(1)[OF s''_is(2)] using alloc_mem_length[OF s''_is(1)] upt_rec
-    by (simp split: prod.splits if_splits)    
+    apply (simp split: prod.splits)
+    apply (metis append_assoc)
+    done
 qed
 
 lemma alloc_globs_range:
@@ -148,7 +161,8 @@ lemma alloc_globs_range:
   shows "i_gs = [length (globs s) ..< (length (globs s) + min (length m_gs) (length vs))] \<and>
          (funcs s) = (funcs s') \<and>
          (tabs s) = (tabs s') \<and>
-         (mems s) = (mems s')"
+         (mems s) = (mems s') \<and>
+         ((globs s)@(map2 (\<lambda>m_g v. \<lparr>g_mut=(tg_mut (module_glob.g_type m_g)), g_val=v\<rparr>) m_gs vs) = (globs s'))"
   using assms
 proof (induction m_gs arbitrary: s i_gs vs)
   case Nil
@@ -172,7 +186,9 @@ next
       by (simp split: prod.splits)
     thus ?thesis
       using outer_Cons(1)[OF s''_is(2)] using alloc_glob_length[OF s''_is(1)] upt_rec Cons
-      by simp
+      apply (simp)
+      apply (metis (no_types, lifting) append_Cons append_assoc self_append_conv2)
+      done
   qed
 qed
 
@@ -383,7 +399,8 @@ definition interp_get_v :: "s \<Rightarrow> inst \<Rightarrow> b_e list \<Righta
 definition interp_get_i32 :: "s \<Rightarrow> inst \<Rightarrow> b_e list \<Rightarrow> i32" where
   "interp_get_i32 s inst b_es = 
      (case interp_get_v s inst b_es of
-        ConstInt32 c \<Rightarrow> c)"
+        ConstInt32 c \<Rightarrow> c
+      | _ \<Rightarrow> 0)"
 
 fun interp_instantiate :: "s \<Rightarrow> m \<Rightarrow> v_ext list \<Rightarrow> ((s \<times> inst \<times> (module_export list)) \<times> (nat option)) option" where
   "interp_instantiate s m v_imps =
@@ -467,41 +484,296 @@ proof (induction "\<C>" "b_es" "([] _> [t])" rule: b_e_typing.induct)
 qed (auto simp add: const_expr.simps)
 
 lemma const_exprs_run_v:
-  assumes "\<C> = \<lparr>types_t=[], func_t=[], global=tgs, table=[], memory=[], local=[], label=[], return=None\<rparr>"
-          "const_exprs \<C> b_es"
+  assumes "const_exprs \<C> b_es"
           "\<C> \<turnstile> b_es : ([] _> [t])"
+          "global \<C> = tgs"
           "list_all2 (\<lambda>ig tg. external_typing s (Ext_glob ig) (Te_glob tg)) igs tgs"
-          "inst = \<lparr>types=arb1,funcs=arb2,tabs=arb3,mems=arb4,globs=igs@arb5\<rparr>"
-  shows "run_v 2 0 inst (s,[],$*b_es) = (s, RValue [v]) \<and> typeof v = t"
-  sorry
+          "inst.globs inst = igs@arb"
+  shows "\<exists>v. typeof v = t \<and> run_v 2 0 inst (s,[],$*b_es) = (s, RValue [v])"
+proof -
+  consider (1) v where "b_es = [C v] \<and> typeof v = t"
+         | (2) j where "b_es = [Get_global j]"
+                       "j < length (global \<C>)"
+                       "tg_mut (global \<C> ! j) = T_immut"
+                       "tg_t (global \<C> ! j) = t"
+    using const_exprs_is[OF assms(1,2)]
+    by blast
+  thus ?thesis
+  proof cases
+    case 1
+    thus ?thesis
+      by (auto simp add: const_list_def is_const_def Suc_1[symmetric])
+  next
+    case 2
+    thus ?thesis
+      using assms
+      unfolding list_all2_conv_all_nth external_typing.simps
+      by (auto simp add: const_list_def is_const_def Suc_1[symmetric] glob_typing_def nth_append sglob_def sglob_ind_def sglob_val_def)
+  qed
+qed
 
 lemma const_exprs_reduce_trans:
-  assumes "\<C> = \<lparr>types_t=[], func_t=[], global=tgs, table=[], memory=[], local=[], label=[], return=None\<rparr>"
-          "const_exprs \<C> b_es"
+  assumes "const_exprs \<C> b_es"
           "\<C> \<turnstile> b_es : ([] _> [t])"
+          "reduce_trans inst_r (s_r,vs,$*b_es) (s',vs',[$C v])"
+          "global \<C> = tgs"
           "list_all2 (\<lambda>ig tg. external_typing s (Ext_glob ig) (Te_glob tg)) igs tgs"
-          "inst = \<lparr>types=arb1,funcs=arb2,tabs=arb3,mems=arb4,globs=igs@arb5\<rparr>"
-          "reduce_trans inst (s,vs,$*b_es) (s',vs',[$C v])"
-  shows "s = s' \<and> vs = vs' \<and> typeof v = t \<and> run_v 2 0 inst (s,[],$*b_es) = (s, RValue [v])"
-  sorry
+          "globs s_r = (globs s)@arbg1"
+          "globs s_v = (globs s)@arbg2"
+          "inst.globs inst_r = igs@arbi1"
+          "inst.globs inst_v = igs@arbi2"
+  shows "s_r = s' \<and> vs = vs' \<and> typeof v = t \<and> run_v 2 0 inst_v (s_v,[],$*b_es) = (s_v, RValue [v])"
+proof -
+  consider (1) v_r where "b_es = [C v_r] \<and> typeof v_r = t"
+         | (2) j where "b_es = [Get_global j]"
+                       "j < length (global \<C>)"
+                       "tg_mut (global \<C> ! j) = T_immut"
+                       "tg_t (global \<C> ! j) = t"
+    using const_exprs_is[OF assms(1,2)]
+    by blast
+  thus ?thesis
+  proof (cases)
+    case 1
+    thus ?thesis
+      using assms(3) reduce_trans_consts
+      apply (simp add: const_list_def is_const_def Suc_1[symmetric])
+      apply (metis (mono_tags, lifting) append_Nil2 case_prod_conv list.inject split_vals_e.simps(1,2) split_vals_e_conv_app)
+      done
+  next
+    case 2
+    have type_is:"typeof (sglob_val s inst_r j) = t" "j < length igs" "(igs!j) < length (globs s)"
+      using assms(4,5,6,8) 2(2,3,4)
+      unfolding list_all2_conv_all_nth external_typing.simps
+      by (simp_all add: glob_typing_def nth_append sglob_def sglob_ind_def sglob_val_def)
+    show ?thesis
+      using assms(3)
+      unfolding reduce_trans_def
+    proof (cases rule: converse_rtranclpE)
+      case base
+      thus ?thesis
+        using 2(1)
+        by auto
+    next
+      case (step y)
+      then obtain s_y vs_y es_y where y_is:"\<lparr>s_r;vs;[$Get_global j]\<rparr> \<leadsto>_ inst_r \<lparr>s_y;vs_y;es_y\<rparr>" "y = (s_y, vs_y, es_y)"
+        using 2
+        by fastforce
+      hence "s_y = s_r \<and> vs_y = vs \<and> es_y = [$C sglob_val s inst_r j]"
+        using assms(6,8)
+      proof (induction s_r vs "[$Get_global j]" inst_r s_y vs_y es_y arbitrary: y rule: reduce.induct)
+        case (basic e' s vs i)
+        thus ?case
+          using lfilled_single
+          apply cases
+          apply auto
+          done
+      next
+        case (get_global s vs i)
+        thus ?case
+          using type_is(2,3)
+          by (simp_all add: sglob_def sglob_ind_def sglob_val_def nth_append)
+      next
+        case (label s vs es i s' vs' es' k lholed les')
+        thus ?case
+          using lfilled_single[OF label(3)]
+          by (metis Lfilled_exact.L0 Lfilled_exact_imp_Lfilled e.distinct(5) lfilled_eq reduce_not_nil)
+      qed auto
+      thus ?thesis
+        using step(2) y_is reduce_trans_consts[of inst_r s_y vs_y "[sglob_val s inst_r j]" s' vs' "[v]"] 2 type_is
+        by (auto simp add: assms(7,8,9) nth_append sglob_def sglob_ind_def sglob_val_def reduce_trans_def const_list_def is_const_def Suc_1[symmetric] split: prod.splits)
+    qed
+  qed
+qed
 
-lemma const_exprs_inst:
-  assumes "\<C> = \<lparr>types_t=[], func_t=[], global=tgs, table=[], memory=[], local=[], label=[], return=None\<rparr>"
-          "const_expr \<C> b_e"
+lemma ext_globs_ind:
+  assumes "i<length (ext_globs v_imps)"
+  shows "\<exists>j. j < length v_imps \<and> Ext_glob ((ext_globs v_imps) ! i) = v_imps!j"
+  using assms
+proof (induction v_imps arbitrary: i)
+case Nil
+  thus ?case
+    by (simp add: map_filter_simps(2))
+next
+  case (Cons v_imp v_imps)
+  consider (1) k where "v_imp = Ext_glob k" | (2) "\<And>k. v_imp \<noteq> Ext_glob k"
+    by blast
+  thus ?case
+  proof (cases)
+    case 1
+    show ?thesis
+    proof (cases i)
+      case 0
+      thus ?thesis
+        using 1
+        by (auto simp add: map_filter_def)
+    next
+      case (Suc i')
+      hence Suc1:"i' < length (ext_globs (v_imps))"
+        using 1 Cons(2)
+        by (simp add: map_filter_def)
+      thus ?thesis
+        using Cons(1)[OF Suc1] Suc 1
+        by (auto simp add: map_filter_def)
+    qed
+  next
+    case 2
+    hence a2:"ext_globs v_imps = ext_globs (v_imp#v_imps)"
+      apply (cases v_imp)
+      apply (simp_all add: map_filter_def)
+      done
+    hence b2:"i < length (ext_globs (v_imps))"
+      using Cons(2)
+      by simp
+    thus ?thesis
+      using Cons(1)[OF b2] a2
+      by auto
+  qed
+qed
+
+lemma alloc_glob_ext_typing:
+  assumes "alloc_glob s (m_g, v) = (s', i_g)"
+          "typeof v = (tg_t (g_type m_g))"
+  shows "external_typing s' (Ext_glob i_g) (Te_glob (g_type m_g))"
+  using assms alloc_glob_length[OF assms(1)]
+  unfolding alloc_glob_def external_typing.simps glob_typing_def
+  apply simp
+  apply (metis global.select_convs(1) global.select_convs(2) nth_append_length)
+  done
+
+lemma alloc_globs_ext_typing:
+  assumes "alloc_globs s m_gs vs = (s', i_gs)"
+          "list_all2 (\<lambda>v m_g. typeof v = (tg_t (g_type m_g))) vs m_gs"
+  shows "list_all2 (\<lambda>ig tg. external_typing s' (Ext_glob ig) (Te_glob tg)) i_gs (map g_type m_gs)"
+  using assms(2,1)
+proof (induction arbitrary: s i_gs rule: list_all2_induct)
+case Nil
+  thus ?case
+    by simp
+next
+  case (Cons x xs y ys)
+  obtain i_g i_gs' s'' where i_gs_is:"i_gs = i_g#i_gs'"
+                                     "alloc_glob s (y,x) = (s'', i_g)"
+                                     "alloc_globs s'' ys xs = (s', i_gs')"
+    using Cons(4)
+    by (fastforce split: prod.splits)
+  have "external_typing s' (Ext_glob i_g) (Te_glob (g_type y))"
+    using alloc_glob_ext_typing[OF i_gs_is(2) Cons(1)] alloc_globs_range[OF i_gs_is(3)] list_all2_lengthD[OF Cons(2)]
+          nth_append[of "s.globs s''"]
+    unfolding external_typing.simps
+    apply simp
+    apply (metis length_append trans_less_add1)
+    done
+  thus ?case
+    using alloc_glob_ext_typing[OF i_gs_is(2) Cons(1)] Cons(3)[OF i_gs_is(3)] i_gs_is(1)
+    by (simp split: prod.splits)
+qed
+
+lemma list_all2_external_typing_glob_alloc:
+  assumes "list_all2 (\<lambda>i t. external_typing s i t) v_imps t_imps"
+  shows "list_all2 (\<lambda>ig tg. external_typing s (Ext_glob ig) (Te_glob tg)) (ext_globs v_imps) (ext_t_globs t_imps)"
+  using assms
+proof (induction t_imps rule: list_all2_induct)
+  case Nil
+  thus ?case
+    by (simp add: map_filter_simps(2))
+next
+  case (Cons x xs y ys)
+  thus ?case
+  proof (cases rule: external_typing.cases)
+    case (4 i gt)
+    thus ?thesis
+      using Cons
+      by (simp add: map_filter_def)
+  qed (fastforce simp add: map_filter_def)+
+qed
+
+lemma alloc_module_ext_arb:
+  assumes "alloc_module s m imps gvs (s',inst,exps)"
+  shows "\<exists>farbs tarbs marbs garbs.
+           (funcs s)@farbs = funcs s' \<and>
+           (tabs s)@tarbs = tabs s' \<and>
+           (mems s)@marbs = mems s' \<and>
+           (globs s)@garbs = globs s'"
+proof -
+  obtain s1 s2 s3 i_fs i_ts i_ms i_gs where inst_is:
+    "inst = \<lparr>types=(m_types m),
+           funcs=(ext_funcs imps)@i_fs,
+           tabs=(ext_tabs imps)@i_ts,
+           mems=(ext_mems imps)@i_ms,
+           globs=(ext_globs imps)@i_gs\<rparr>"
+    "alloc_funcs s (m_funcs m) inst = (s1,i_fs)"
+    "alloc_tabs s1 (m_tabs m) = (s2,i_ts)"
+    "alloc_mems s2 (m_mems m) = (s3,i_ms)"
+    "alloc_globs s3 (m_globs m) gvs = (s',i_gs)"
+    "exps = map (\<lambda>m_exp. \<lparr>E_name=(E_name m_exp), E_desc=(export_get_v_ext inst (E_desc m_exp))\<rparr>) (m_exports m)"
+    using assms(1)
+    unfolding alloc_module.simps
+    by blast
+  show ?thesis
+    using alloc_funcs_range[OF inst_is(2)]
+          alloc_tabs_range[OF inst_is(3)]
+          alloc_mems_range[OF inst_is(4)]
+          alloc_globs_range[OF inst_is(5)]
+    by fastforce
+qed
+
+lemma alloc_module_external_typing_preserved:
+  assumes "alloc_module s m imps gvs (s',inst,exps)"
+          "external_typing s v_imp t_imp"
+  shows "external_typing s' v_imp t_imp"
+  using assms(2,1)
+proof (cases rule: external_typing.cases)
+  case (1 i tf)
+  thus ?thesis
+    using alloc_module_ext_arb[OF assms(1)]
+    by (metis add.commute external_typing.intros(1) length_append nth_append trans_less_add2)
+next
+  case (2 i tt)
+  thus ?thesis
+    using alloc_module_ext_arb[OF assms(1)]
+    by (metis external_typing.intros(2) length_append nth_append trans_less_add1)
+next
+  case (3 i mt)
+  thus ?thesis
+    using alloc_module_ext_arb[OF assms(1)]
+    by (metis external_typing.intros(3) length_append nth_append trans_less_add1)
+next
+  case (4 i gt)
+  thus ?thesis
+    using alloc_module_ext_arb[OF assms(1)]
+    by (metis external_typing.intros(4) length_append nth_append trans_less_add1)
+qed
+
+lemma g_init_type:
+  assumes "interp_get_v s inst (g_init m_g) = gv"
+          "(module_glob_typing \<C>) m_g gt"
+          "global \<C> = tgs"
           "list_all2 (\<lambda>ig tg. external_typing s (Ext_glob ig) (Te_glob tg)) igs tgs"
-          "inst = \<lparr>types=[],funcs=[],tabs=[],mems=[],globs=igs\<rparr>"
-          "inst' = \<lparr>types=arb1,funcs=arb2,tabs=arb3,mems=arb4,globs=igs@arb5\<rparr>"
-  shows "\<lparr>s;vs;[$b_e]\<rparr> \<leadsto>_inst \<lparr>s;vs;[$C v]\<rparr> = \<lparr>s;vs;[$b_e]\<rparr> \<leadsto>_inst' \<lparr>s;vs;[$C v]\<rparr>"
-  sorry
+          "inst.globs inst = igs@arb"
+  shows "typeof gv = tg_t (g_type m_g)"
+proof -
+  have 1:"const_exprs \<C> (g_init m_g)"
+    using assms(2)
+    unfolding module_glob_typing.simps
+    by fastforce
+  have 2:"\<C> \<turnstile> (g_init m_g) : ([] _> [tg_t (g_type m_g)])"
+    using assms(2)
+    unfolding module_glob_typing.simps
+    by fastforce
+  show ?thesis
+    using const_exprs_run_v[OF 1 2 assms(3,4,5)] assms(1)
+    unfolding interp_get_v_def
+    by (simp split: prod.splits)
+qed
 
 lemma interp_instantiate_imp_instantiate:
   assumes "(interp_instantiate s m v_imps = Some ((s_end, inst, v_exps), start))"
   shows "(instantiate s m v_imps ((s_end, inst, v_exps), start))"
 proof -
-  obtain t_imps t_exps g_inits s' e_offs d_offs s'' where m_is:
+  obtain t_imps t_exps g_inits s' e_offs d_offs s'' inst' where s_end_is:
     "module_type_checker m = Some (t_imps, t_exps)"
     "(list_all2 (external_typing s) v_imps t_imps)"
-    "g_inits = map (\<lambda>g. interp_get_v s \<lparr>types=[],funcs=[],tabs=[],mems=[],globs=ext_globs v_imps\<rparr> (g_init g)) (m_globs m)"
+    "g_inits = map (\<lambda>g. interp_get_v s inst' (g_init g)) (m_globs m)"
     "(s', inst, v_exps) = interp_alloc_module s m v_imps g_inits"
     "e_offs = map (\<lambda>e. interp_get_i32 s' inst (e_off e)) (m_elem m)"
     "d_offs = map (\<lambda>d. interp_get_i32 s' inst (d_off d)) (m_data m)"
@@ -510,21 +782,343 @@ proof -
     "start = map_option (\<lambda>i_s. ((inst.funcs inst)!i_s)) (m_start m)"
     "s'' = init_tabs s' inst (map nat_of_int e_offs) (m_elem m)"
     "s_end = init_mems s' inst (map nat_of_int d_offs) (m_data m)"
+    "inst' = \<lparr>types=[],funcs=[],tabs=[],mems=[],globs=ext_globs v_imps\<rparr>"
     using assms
     by (fastforce simp add: Let_def split: if_splits option.splits prod.splits)
 
   have 1:"module_typing m t_imps t_exps"
-    using m_is(1) module_type_checker_imp_module_typing
+    using s_end_is(1) module_type_checker_imp_module_typing
     by blast
   have 2:"alloc_module s m v_imps g_inits (s', inst, v_exps)"
-    using m_is(4) interp_alloc_module_imp_alloc_module
+    using s_end_is(4) interp_alloc_module_imp_alloc_module
     by metis
-  have 3:"list_all2 (\<lambda>g v. reduce_trans inst (s',[],$*(g_init g)) (s',[],[$C v])) (m_globs m) g_inits"
-         "list_all2 (\<lambda>e c. reduce_trans inst (s',[],$*(e_off e)) (s',[],[$C ConstInt32 c])) (m_elem m) e_offs"
-         "list_all2 (\<lambda>d c. reduce_trans inst (s',[],$*(d_off d)) (s',[],[$C ConstInt32 c])) (m_data m) d_offs"
-    sorry
-  show ?thesis
-    using instantiate.intros[OF 1 m_is(2) 2 3 m_is(7,8) m_is(9,10,11)[symmetric]]
+
+  obtain fs fts ts ms gs gts els ds i_opt imps exps tfs ifts itts imts igts \<C> \<C>' where m_is:
+    "list_all2 (module_func_typing \<C>) fs fts"
+    "list_all (module_tab_typing) ts"
+    "list_all (module_mem_typing) ms"
+    "list_all2 (module_glob_typing \<C>') gs gts"
+    "list_all (module_elem_typing \<C>) els"
+    "list_all (module_data_typing \<C>) ds"
+    "pred_option (module_start_typing \<C>) i_opt"
+    "list_all2 (\<lambda>imp. module_import_typing \<C> (I_desc imp)) imps t_imps"
+    "list_all2 (\<lambda>exp. module_export_typing \<C> (E_desc exp)) exps t_exps"
+    "ifts = ext_t_funcs t_imps"
+    "itts = ext_t_tabs t_imps"
+    "imts = ext_t_mems t_imps"
+    "igts = ext_t_globs t_imps"
+    "\<C> = \<lparr>types_t=tfs, func_t=ifts@fts, global=igts@gts, table=itts@ts, memory=imts@ms, local=[], label=[], return=None\<rparr>"
+    "\<C>' = \<lparr>types_t=[], func_t=[], global=igts, table=[], memory=[], local=[], label=[], return=None\<rparr>"
+    "m = \<lparr>m_types = tfs,
+          m_funcs = fs,
+          m_tabs = ts,
+          m_mems = ms,
+          m_globs = gs,
+          m_elem = els,
+          m_data = ds,
+          m_start = i_opt,
+          m_imports = imps,
+          m_exports = exps\<rparr>"
+    using 1
+    unfolding module_typing.simps
     by blast
+
+  obtain s1 s2 s3 i_fs i_ts i_ms i_gs where inst_is:
+    "inst = \<lparr>types=(m_types m),
+           funcs=(ext_funcs v_imps)@i_fs,
+           tabs=(ext_tabs v_imps)@i_ts,
+           mems=(ext_mems v_imps)@i_ms,
+           globs=(ext_globs v_imps)@i_gs\<rparr>"
+    "alloc_funcs s (m_funcs m) inst = (s1,i_fs)"
+    "alloc_tabs s1 (m_tabs m) = (s2,i_ts)"
+    "alloc_mems s2 (m_mems m) = (s3,i_ms)"
+    "alloc_globs s3 (m_globs m) g_inits = (s',i_gs)"
+    "v_exps = map (\<lambda>m_exp. \<lparr>E_name=(E_name m_exp), E_desc=(export_get_v_ext inst (E_desc m_exp))\<rparr>) (m_exports m)"
+    using 2
+    unfolding alloc_module.simps
+    by blast
+
+  have 12:"list_all2 (\<lambda>ig tg. external_typing s (Ext_glob ig) (Te_glob tg)) (inst.globs inst') (global \<C>')"
+    using s_end_is(2,12) m_is(13,15) ext_globs_ind list_all2_external_typing_glob_alloc
+    by simp
+  have 11:"list_all2 (\<lambda>ig tg. external_typing s' (Ext_glob ig) (Te_glob tg)) (inst.globs inst) (global \<C>)"
+  proof -
+    have "list_all2 (\<lambda>ig tg. external_typing s' (Ext_glob ig) (Te_glob tg)) (inst.globs inst') (global \<C>')"
+      using alloc_module_external_typing_preserved[OF 2] 12
+      unfolding list_all2_conv_all_nth
+      by fastforce
+    moreover
+    have 111:"list_all2 (\<lambda>v m_g. typeof v = tg_t (g_type m_g)) g_inits (m_globs m)"
+      using s_end_is(3)[symmetric] g_init_type[OF _ _ _ 12, of inst' _ _ \<C>' _ "[]"] m_is(4,16)
+      by (auto simp add: list_all2_conv_all_nth)
+    have "(gather_m_g_types (m_globs m)) = gts"
+      using m_is(4,16)
+      unfolding list_all2_conv_all_nth module_glob_typing.simps
+      apply simp
+      apply (metis length_map module_glob.select_convs(1) nth_equalityI nth_map)
+      done
+    hence "list_all2 (\<lambda>ig tg. external_typing s' (Ext_glob ig) (Te_glob tg)) i_gs gts"
+      using alloc_globs_ext_typing[OF inst_is(5) 111]
+      by blast
+    ultimately
+    show ?thesis
+      using list_all2_appendI
+      by (fastforce simp add: m_is(14,15) inst_is(1) s_end_is(12))
+  qed
+
+  have 3:"list_all2 (\<lambda>g v. reduce_trans inst (s',[],$*(g_init g)) (s',[],[$C v])) (m_globs m) g_inits"
+  proof -
+    { fix i
+      assume local_assms:"length (m_globs m) = length g_inits" "i<length (m_globs m)"
+      hence l1:"const_exprs \<C>' (g_init (m_globs m ! i))"
+        using m_is(4,16)
+        unfolding list_all2_conv_all_nth module_glob_typing.simps
+        by auto
+      obtain t where l2:"\<C>' \<turnstile> (g_init (m_globs m ! i)) : ([] _> [t])"
+        using local_assms m_is(4,16)
+        unfolding list_all2_conv_all_nth module_glob_typing.simps
+        by auto
+      obtain v_r where "run_v 2 0 inst' (s, [], $* (g_init (m_globs m ! i))) =  (s, RValue [v_r])"
+        using const_exprs_run_v[OF l1 l2 _ 12, of inst']
+        by auto
+      hence "run_v 2 0 inst' (s,[],$*(g_init ((m_globs m)!i))) = (s,RValue [(g_inits!i)])"
+        using s_end_is(3) local_assms
+        by (simp add: interp_get_v_def split: v.splits)
+      hence l3:"reduce_trans inst' (s,[],$*(g_init ((m_globs m)!i))) (s,[],[$C (g_inits!i)])"
+        using reduce_trans_length_locals run_v_sound
+        by fastforce
+      obtain arbg arbi where arbgi:"(globs s)@arbg = (globs s')"
+                                   "inst.globs inst = inst.globs inst' @ arbi"
+        using alloc_module_ext_arb[OF 2] 2 s_end_is(12)
+        unfolding alloc_module.simps
+        by auto
+      have "run_v 2 0 inst (s', [], $* g_init (m_globs m ! i)) = (s', RValue [g_inits ! i])"
+        using const_exprs_reduce_trans[OF l1 l2 l3 _ 12 _ arbgi(1)[symmetric] _ arbgi(2)]
+        by fastforce
+      hence "reduce_trans inst (s',[],$*(g_init ((m_globs m)!i))) (s',[],[$C (g_inits!i)])"
+        using reduce_trans_length_locals run_v_sound
+        by fastforce
+    }
+    thus ?thesis
+      using s_end_is(3)
+      unfolding list_all2_conv_all_nth
+      by fastforce
+  qed
+
+  have 4:"list_all2 (\<lambda>e c. reduce_trans inst (s',[],$*(e_off e)) (s',[],[$C ConstInt32 c])) (m_elem m) e_offs"
+  proof -
+    { fix i
+      assume local_assms:"length (m_elem m) = length e_offs" "i<length (m_elem m)"
+      hence l1:"const_exprs \<C> (e_off (m_elem m ! i))"
+        by (metis m_is(5,16) list_all_length m.select_convs(6) module_elem.select_convs(2) module_elem_typing.cases)
+      have l2:"\<C> \<turnstile> (e_off (m_elem m ! i)) : ([] _> [T_i32])"
+        using local_assms
+        by (metis m_is(5,16) list_all_length m.select_convs(6) module_elem.select_convs(2) module_elem_typing.cases)
+      obtain c_r where "run_v 2 0 inst (s', [], $* e_off (m_elem m ! i)) =  (s', RValue [ConstInt32 c_r])"
+        using const_exprs_run_v[OF l1 l2 _ 11, of inst "[]"] typeof_i32
+        by auto
+      hence "run_v 2 0 inst (s', [], $* e_off (m_elem m ! i)) = (s', RValue [ConstInt32 (e_offs ! i)])"
+        using s_end_is(5) local_assms
+        by (simp add: interp_get_i32_def interp_get_v_def split: v.splits)
+      hence "reduce_trans inst (s', [], $* e_off (m_elem m ! i)) (s', [], [$C ConstInt32 (e_offs ! i)])"
+        using reduce_trans_length_locals run_v_sound
+        by fastforce
+    }
+    thus ?thesis
+      using s_end_is(5)
+      unfolding list_all2_conv_all_nth
+      by fastforce
+  qed
+  have 5:"list_all2 (\<lambda>d c. reduce_trans inst (s',[],$*(d_off d)) (s',[],[$C ConstInt32 c])) (m_data m) d_offs"
+  proof -
+    { fix i
+      assume local_assms:"length (m_data m) = length d_offs" "i<length (m_data m)"
+      hence l1:"const_exprs \<C> (d_off (m_data m ! i))"
+        by (metis list_all_length m.select_convs(7) m_is(6,16) module_data.select_convs(2) module_data_typing.simps)
+      have l2:"\<C> \<turnstile> (d_off (m_data m ! i)) : ([] _> [T_i32])"
+        using local_assms
+        by (metis list_all_length m.select_convs(7) m_is(6,16) module_data.select_convs(2) module_data_typing.simps)
+      obtain c_r where "run_v 2 0 inst (s', [], $* d_off (m_data m ! i)) =  (s', RValue [ConstInt32 c_r])"
+        using const_exprs_run_v[OF l1 l2 _ 11, of inst "[]"] typeof_i32
+        by auto
+      hence "run_v 2 0 inst (s', [], $* d_off (m_data m ! i)) = (s', RValue [ConstInt32 (d_offs ! i)])"
+        using s_end_is(6) local_assms
+        by (simp add: interp_get_i32_def interp_get_v_def split: v.splits)
+      hence "reduce_trans inst (s', [], $* d_off (m_data m ! i)) (s', [], [$C ConstInt32 (d_offs ! i)])"
+        using reduce_trans_length_locals run_v_sound
+        by fastforce
+    }
+    thus ?thesis
+      using s_end_is(6)
+      unfolding list_all2_conv_all_nth
+      by fastforce
+   qed
+   show ?thesis
+    using instantiate.intros[OF 1 s_end_is(2) 2 3 4 5 s_end_is(7,8) s_end_is(9,10,11)[symmetric]]
+    by blast
+qed
+
+lemma map_intro_length:
+  assumes "\<And>i. i < length ls \<Longrightarrow> F (ls!i) = fls!i"
+          "length ls = length fls"
+  shows "map F ls = fls"
+  using assms
+  by (metis length_map nth_equalityI nth_map)
+
+lemma instantiate_imp_interp_instantiate:
+  assumes "(instantiate s m v_imps ((s_end, inst, v_exps), start))"
+  shows "(interp_instantiate s m v_imps = Some ((s_end, inst, v_exps), start))"
+proof -
+  obtain fs ts ms gs els ds i_opt imps exps tfs where m_is:
+    "m = \<lparr>m_types = tfs,
+          m_funcs = fs,
+          m_tabs = ts,
+          m_mems = ms,
+          m_globs = gs,
+          m_elem = els,
+          m_data = ds,
+          m_start = i_opt,
+          m_imports = imps,
+          m_exports = exps\<rparr>"
+    using m.cases
+    by blast
+  obtain inst' where inst'_is:
+    "inst' = \<lparr>types=[],funcs=[],tabs=[],mems=[],globs=ext_globs v_imps\<rparr>"
+    using inst.cases
+    by blast
+
+  obtain t_imps t_exps g_inits s' e_offs d_offs s'' where s_end_is:
+    "module_typing m t_imps t_exps"
+    "list_all2 (external_typing s) v_imps t_imps"
+    "alloc_module s m v_imps g_inits (s', inst, v_exps)"
+    "list_all2 (\<lambda>g v. reduce_trans inst (s',[],$*(g_init g)) (s',[],[$C v])) gs g_inits"
+    "list_all2 (\<lambda>e c. reduce_trans inst (s',[],$*(e_off e)) (s',[],[$C ConstInt32 c])) els e_offs"
+    "list_all2 (\<lambda>d c. reduce_trans inst (s',[],$*(d_off d)) (s',[],[$C ConstInt32 c])) ds d_offs"
+    "list_all2 (\<lambda>e_off e. ((nat_of_int e_off) + (length (e_init e))) \<le> length (fst ((tabs s)!((inst.tabs inst)!(e_tab e))))) e_offs els"
+    "list_all2 (\<lambda>d_off d. ((nat_of_int d_off) + (length (d_init d))) \<le> mem_length ((mems s)!((inst.mems inst)!(d_data d)))) d_offs ds"
+    "map_option (\<lambda>i_s. ((inst.funcs inst)!i_s)) i_opt = start"
+    "init_tabs s' inst (map nat_of_int e_offs) els = s''"
+    "init_mems s' inst (map nat_of_int d_offs) ds = s_end"
+    using assms m_is
+    unfolding instantiate.simps
+    by fastforce
+
+  obtain fts gts ifts itts imts igts \<C> \<C>' where m_is_2:
+    "list_all2 (module_func_typing \<C>) fs fts"
+    "list_all (module_tab_typing) ts"
+    "list_all (module_mem_typing) ms"
+    "list_all2 (module_glob_typing \<C>') gs gts"
+    "list_all (module_elem_typing \<C>) els"
+    "list_all (module_data_typing \<C>) ds"
+    "pred_option (module_start_typing \<C>) i_opt"
+    "list_all2 (\<lambda>imp. module_import_typing \<C> (I_desc imp)) imps t_imps"
+    "list_all2 (\<lambda>exp. module_export_typing \<C> (E_desc exp)) exps t_exps"
+    "ifts = ext_t_funcs t_imps"
+    "itts = ext_t_tabs t_imps"
+    "imts = ext_t_mems t_imps"
+    "igts = ext_t_globs t_imps"
+    "\<C> = \<lparr>types_t=tfs, func_t=ifts@fts, global=igts@gts, table=itts@ts, memory=imts@ms, local=[], label=[], return=None\<rparr>"
+    "\<C>' = \<lparr>types_t=[], func_t=[], global=igts, table=[], memory=[], local=[], label=[], return=None\<rparr>"
+    using s_end_is(1) m_is
+    unfolding module_typing.simps
+    by blast
+
+  have 12:"list_all2 (\<lambda>ig tg. external_typing s (Ext_glob ig) (Te_glob tg)) (inst.globs inst') (global \<C>')"
+    using ext_globs_ind list_all2_external_typing_glob_alloc
+    by (simp add: inst'_is m_is_2(13,15) s_end_is(2))
+  have 11:"list_all2 (\<lambda>ig tg. external_typing s' (Ext_glob ig) (Te_glob tg)) (inst.globs inst) (global \<C>)"
+    sorry
+
+  have "(module_type_checker m) = Some (t_imps, t_exps)"
+    using s_end_is(1) module_typing_equiv_module_type_checker
+    by blast
+  moreover
+  have "g_inits = map (\<lambda>g. interp_get_v s inst' (g_init g)) gs"
+  proof -
+    { fix i
+      assume local_assms: "i < length gs"
+      obtain t where l2:"\<C>' \<turnstile> (g_init (gs ! i)) : ([] _> [t])"
+                        "const_exprs \<C>' (g_init (gs ! i))"
+        using local_assms m_is m_is m_is_2(4,15)
+        unfolding list_all2_conv_all_nth module_glob_typing.simps
+        by auto
+      have l1:"reduce_trans inst (s',[],$*(g_init (gs!i))) (s',[],[$C (g_inits!i)])"
+        using s_end_is(4) local_assms
+        unfolding list_all2_conv_all_nth
+        by blast
+      have "run_v 2 0 inst' (s,[],$*(g_init (gs!i))) = (s,RValue [g_inits!i])"
+        using const_exprs_reduce_trans[OF l2(2,1) l1 _ 12, of _ s "[]" _ inst' "[]"]
+              alloc_module_ext_arb[OF s_end_is(3)] s_end_is(3)
+        unfolding alloc_module.simps
+        apply simp
+        apply (metis (mono_tags, lifting) inst'_is inst.select_convs(5))
+        done
+      hence "interp_get_v s inst' (g_init (gs!i)) = g_inits!i"
+        unfolding interp_get_v_def
+        by fastforce
+    }
+    thus ?thesis
+      using map_intro_length[symmetric, of gs "(\<lambda>g. interp_get_v s inst' (g_init g))" g_inits]
+            list_all2_lengthD[OF s_end_is(4)]
+      by fastforce
+  qed
+  moreover
+  have "interp_alloc_module s m v_imps g_inits = (s', inst, v_exps)"
+    using s_end_is(3) alloc_module_equiv_interp_alloc_module
+    by blast
+  moreover
+  have "e_offs = map (\<lambda>e. interp_get_i32 s' inst (e_off e)) els"
+  proof -
+    { fix i
+      assume local_assms: "i < length els"
+      have l2:"const_exprs \<C> (e_off (els ! i))"
+              "\<C> \<turnstile> e_off (els ! i) : ([] _> [T_i32])"
+        using m_is_2(5)
+        by (metis list_all_length local_assms module_elem.select_convs(2) module_elem_typing.cases)+
+      have l1:"reduce_trans inst (s',[],$*(e_off (els!i))) (s',[],[$C ConstInt32 (e_offs!i)])"
+        using s_end_is(5) local_assms
+        unfolding list_all2_conv_all_nth
+        by blast
+      have "run_v 2 0 inst (s',[],$*(e_off (els!i))) = (s',RValue [ConstInt32 (e_offs!i)])"
+        using const_exprs_reduce_trans[OF l2(1,2) l1 _ 11]
+        by fastforce
+      hence "interp_get_i32 s' inst (e_off (els!i)) = e_offs!i"
+        unfolding interp_get_i32_def interp_get_v_def
+        by fastforce
+    }
+    thus ?thesis
+      using map_intro_length[symmetric, of els "(\<lambda>e. interp_get_i32 s' inst (e_off e))" e_offs]
+            list_all2_lengthD[OF s_end_is(5)]
+      by fastforce
+  qed
+  moreover
+  have "d_offs = map (\<lambda>d. interp_get_i32 s' inst (d_off d)) ds"
+  proof -
+    { fix i
+      assume local_assms: "i < length ds"
+      have l2:"const_exprs \<C> (d_off (ds ! i))"
+              "\<C> \<turnstile> d_off (ds ! i) : ([] _> [T_i32])"
+        using m_is_2(6)
+        by (metis list_all_length local_assms module_data.select_convs(2) module_data_typing.cases)+
+      have l1:"reduce_trans inst (s',[],$*(d_off (ds!i))) (s',[],[$C ConstInt32 (d_offs!i)])"
+        using s_end_is(6) local_assms
+        unfolding list_all2_conv_all_nth
+        by blast
+      have "run_v 2 0 inst (s',[],$*(d_off (ds!i))) = (s',RValue [ConstInt32 (d_offs!i)])"
+        using const_exprs_reduce_trans[OF l2(1,2) l1 _ 11]
+        by fastforce
+      hence "interp_get_i32 s' inst (d_off (ds!i)) = d_offs!i"
+        unfolding interp_get_i32_def interp_get_v_def
+        by fastforce
+    }
+    thus ?thesis
+      using map_intro_length[symmetric, of ds "(\<lambda>e. interp_get_i32 s' inst (d_off e))" d_offs]
+            list_all2_lengthD[OF s_end_is(6)]
+      by fastforce
+  qed
+  ultimately
+  show ?thesis
+    using s_end_is(2,7,8,9,10,11) m_is inst'_is
+    by simp
 qed
 end
